Isabelle/Composition.thy
@@ -3,7 +3,7 @@ imports ComposableGC "/home/nano/Documents/IO-Automata/Simulations" "~~/src/HOL/
 begin
 
 datatype ('a,'c,'l) comp_action = 
-  Propose1 'c 
+  Propose1 'c
 | Propose2 'c
 | Learn1 'a 'l
 | Learn2 'a 'l
@@ -52,189 +52,182 @@ definition composition where
 definition spec where
   "spec \<equiv> rename initial rn3"
 
-definition inv1 where
+named_theorems inv_defs 
+
+definition inv1::"('a,'b,'c)cgc_state \<times> ('a,'b,'c)cgc_state \<Rightarrow> bool" where
   "inv1 r \<equiv> let r1 = fst r; r2 = snd r in
     (\<forall> s \<in> cgc_state.fromPrev r2 . \<forall> l . \<forall> s' \<in> learned r1 l . s' \<preceq> s)"
+declare inv1_def[inv_defs]
 
-definition inv2 where
+definition inv2::"('a,'b,'c)cgc_state \<times> ('a,'b,'c)cgc_state \<Rightarrow> bool" where
   "inv2 r \<equiv> let r1 = fst r; r2 = snd r in 
     cgc_state.fromPrev r2 = cgc_state.toNext r1"
+declare inv2_def[inv_defs]
 
 definition inv3 where
   "inv3 r \<equiv> let r1 = fst r; r2 = snd r in
     cgc_state.fromPrev r1 = {\<bottom>}"
+declare inv3_def[inv_defs]
 
 definition inv4 where
   "inv4 r \<equiv> let r1 = fst r; r2 = snd r in
     \<forall> l . \<forall> s \<in> learned r2 l . \<exists> s' \<in> cgc_state.fromPrev r2 . s' \<preceq> s"
+declare inv4_def[inv_defs]
 
 definition inv5 where
   "inv5 r \<equiv> let r1 = fst r; r2 = snd r in
     \<forall> s \<in> cgc_state.toNext r2 . \<exists> s' \<in> cgc_state.fromPrev r2 . s' \<preceq> s"
+declare inv5_def[inv_defs]
 
-lemmas defs1 = composition_def par2_def asig_comp2_def cgc_ioa_def rename_def cgc_start_def
-    rename_set_def cgc_asig_def is_trans_def actions_def cgc_trans_def initial_def hide_def propose_def learn_def fromPrev_def toNext_def
+definition inv6 where
+  "inv6 r \<equiv> let r1 = fst r; r2 = snd r in
+    \<forall> s  \<in> cgc_state.toNext r1 . s \<in> non_trivial r1"
+declare inv6_def[inv_defs]
+
+lemmas cgc_ioa_defs = composition_def par2_def asig_comp2_def cgc_ioa_def rename_def
+    rename_set_def cgc_asig_def is_trans_def actions_def cgc_trans_def initial_def hide_def 
+    propose_def 
+lemmas actions_defs = learn_def fromPrev_def toNext_def
     hide_asig_def externals_def cgc_start_def spec_def
-
 lemmas ref_defs = refines_def actions_def trace_def schedule_def filter_act_def
 
+named_theorems invs
+named_theorems mydefs
+declare cgc_ioa_defs[mydefs]
+declare actions_defs[mydefs]
+
+method bring_invs =
+  -- "bring all the invariants in the premises"
+  ( (insert invs) -- "insert invariant theorems in the premises; 
+      this will allow us to use [thin] to get rid of them after use",
+    ( (match premises in I[thin]:"invariant composition ?inv"
+        and R:"reachable composition ?s" \<Rightarrow> 
+            \<open>insert I[simplified invariant_def, rule_format, OF R]\<close>)+
+        -- "for each invariant theorem, use the reachability assumption to obtain the invariant",
+      (match premises in R[thin]:"reachable composition ?s" \<Rightarrow> succeed)
+        -- "finally get rid of the reachability assumption"
+        )? -- "don't fail if there are no invariants to bring"
+    )
+
+method try_solve_inv declares mydefs =
+  ( rule invariantI, 
+    force simp add:mydefs inv_defs -- "solve the base case",
+    bring_invs,
+    match premises in T:"?s \<midarrow>a\<midarrow>composition\<longrightarrow> ?t" for a \<Rightarrow> \<open>case_tac a\<close> 
+      -- "do case analysis on the action";
+    auto simp add:mydefs inv_defs)
+
 lemma inv2:"invariant composition inv2"
-apply (rule invariantI)
-  apply(simp add:defs1 inv2_def)
-  apply(case_tac "a")
-  apply(auto simp add:defs1 inv2_def)
-done
+  by try_solve_inv
+declare inv2[invs]
 
 lemma inv1:"invariant composition inv1"
-apply (rule invariantI)
-  apply(simp add:defs1 inv1_def )
-  apply(drule_tac inv2[simplified invariant_def, rule_format])
-  apply(case_tac "a")
-  apply(auto simp add:defs1 inv1_def inv2_def non_trivial_def)
-done
+  by try_solve_inv
+declare inv1[invs]
 
 lemma inv3:"invariant composition inv3"
-apply (rule invariantI)
-  apply(simp add:defs1 inv3_def)
-  apply(case_tac "a")
-  apply(auto simp add:defs1 inv3_def)
-done
+  by try_solve_inv
+declare inv3[invs]
 
 lemma inv4:"invariant composition inv4"
-apply (rule invariantI)
-  apply(simp add:defs1 inv4_def)
-  apply(case_tac "a")
-  apply(thin_tac "reachable composition s")
-  apply(auto simp add:defs1 inv4_def non_trivial_def less_eq_def)
-done
+  by (try_solve_inv mydefs:non_trivial_def less_eq_def)
+declare inv4[invs]
 
 lemma inv5:"invariant composition inv5"
-apply (rule invariantI)
-  apply(simp add:defs1 inv5_def)
-  apply(case_tac "a")
-  apply(thin_tac "reachable composition s")
-  apply(auto simp add:defs1 inv5_def non_trivial_def less_eq_def)
-done
+  by (try_solve_inv mydefs:non_trivial_def less_eq_def)
+declare inv5[invs]
 
-lemmas inv11 = inv1[simplified invariant_def]
-thm inv11[split_format(complete)]
-lemmas invs[simplified invariant_def, rule_format] = inv1 inv2
+lemma inv6:"invariant composition inv6"
+  apply (try_solve_inv mydefs:non_trivial_def less_eq_def)
+  apply (metis subset_insertI2)
+  done
+declare inv6[invs]
 
-lemma l1:
+named_theorems lems
+
+lemma l1[lems]:
   assumes "s\<^sub>0 \<preceq> s\<^sub>1" and "s\<^sub>2 = s\<^sub>1 \<star> cs"
   shows "compat2 s\<^sub>0 s\<^sub>2"
   using assms
 by (metis less_eq_def local.compat2_def local.trans) 
 
-abbreviation refmap where
+lemma l2[lems]:
+  assumes "s1 = \<bottom> \<star> cs" and "s2 = s1 \<star> cs'"
+  obtains cs'' where "s2 = \<bottom> \<star> cs''" and "set cs'' = set cs \<union> set cs'"
+  using assms
+  by (metis inf_sup_aci(5) pre_CStruct.exec_append set_append)
+
+definition refmap where
   "refmap r \<equiv> let r1 = fst r; r2 = snd r in 
     \<lparr>cgc_state.propCmd = propCmd r1 \<union> propCmd r2, 
       cgc_state.learned = (\<lambda> l . learned r1 l \<union> learned r2 l),
       cgc_state.fromPrev = {\<bottom>}, 
       toNext = cgc_state.toNext r2\<rparr>"
 
-method my_allE for y :: 'a =
-(match premises in I [thin]: "\<forall> x :: 'a. ?Q x" \<Rightarrow>
-  \<open>rule allE [where x = y, OF I ]\<close>)
+method app_fun_eq_iff =
+  (match conclusion in "(\<lambda> x . ?B x) = (\<lambda> x . ?A x)" \<Rightarrow> \<open>simp add:fun_eq_iff\<close>)
 
-method print_inv =
-  match invs in M [thin] :"\<And> s . reachable composition s \<Longrightarrow> ?Inv" \<Rightarrow> \<open>print_fact M\<close>
+method split_conjs =
+  (rule conjI);split_conjs?
 
 lemma refok:"is_ref_map refmap composition spec"
-apply(simp add:is_ref_map_def, rule conjI; clarify)
- apply(simp add:defs1)
+apply(simp add:is_ref_map_def refmap_def, rule conjI; clarify)
+ apply(force simp add:mydefs)
+ apply(bring_invs)
  apply(case_tac ab, auto)
-   apply(thin_tac "reachable composition (a, b)")
+
    apply(rule_tac x="refmap (a,b)" in exI)
    apply(rule_tac x="[(Propose1 x1,refmap (aa,ba))]" in exI)
-   apply(simp add:defs1 ref_defs)
+   apply(force simp add:mydefs ref_defs refmap_def)
 
-   apply(thin_tac "reachable composition (a, b)")
    apply(rule_tac x="refmap (a,b)" in exI)
    apply(rule_tac x="[(Propose2 x2,refmap (aa,ba))]" in exI)
-   apply(simp add:defs1 ref_defs)
-
-   prefer 3
-   apply(thin_tac "reachable composition (a, b)")
-   apply(rule_tac x="refmap (a,b)" in exI)
-   apply(rule_tac x="[]" in exI)
-   apply(simp add:defs1 ref_defs)
+   apply(force simp add:mydefs ref_defs refmap_def)
 
    apply(rule_tac x="refmap (a,b)" in exI)
    apply(rule_tac x="[(Learn1 x31 x32,refmap (aa,ba))]" in exI)
-   apply(frule_tac inv1[simplified invariant_def, rule_format])
-   apply(frule_tac inv3[simplified invariant_def, rule_format])
-   apply(frule_tac inv2[simplified invariant_def, rule_format])
-   apply(frule_tac inv4[simplified invariant_def, rule_format])
-   apply(frule_tac inv5[simplified invariant_def, rule_format])
-   apply(thin_tac "reachable composition (a,b)")
-   proof -
-    fix r1 r2 l r1' r2' s
-    assume learn:"(r1, r2) \<midarrow>Learn1 s l\<midarrow>composition\<longrightarrow> (r1', r2')" and inv1:"inv1 (r1, r2)" and inv2:"inv2 (r1, r2)" and inv3:"inv3 (r1,r2)" and inv4:"inv4 (r1,r2)"
-    and inv5:"inv5 (r1,r2)"
-    show "refines (refmap (r1, r2), [(Learn1 s l, refmap (r1', r2'))]) (r1, r2) (Learn1 s l) (r1', r2') spec refmap"
-    proof -
-      from learn have 1:"learn l s r1 r1'" and 2:"r2 = r2'"
-        by (auto simp add: defs1)
-      have "learn l s (refmap (r1, r2)) (refmap (r1',r2'))"
-      proof -
-        have "s \<in> non_trivial (refmap (r1, r2))" using 1 inv3 
-          by (auto simp add:learn_def inv3_def non_trivial_def)
-        moreover
-        have "cgc_state.fromPrev (refmap (r1, r2)) \<noteq> {}" using inv3
-          by (auto simp add:inv3_def)
-        moreover 
-        have "let learned1 = learned (refmap (r1, r2)) in (refmap (r1', r2')) = (refmap (r1, r2))\<lparr>learned := (learned1(l := learned1 l \<union> {s}))\<rparr>"
-          using 1 2
-          by (auto simp add:learn_def fun_eq_iff)
-        moreover 
-        have "\<forall> l . \<forall> s' \<in> learned (refmap (r1, r2)) l . compat2 s' s"
-        proof auto
-          fix l s'
-          assume "s' \<in> learned r1 l"
-          thus "compat2 s' s" using 1 by (simp add:learn_def)
-        next
-          fix l s'
-          assume 3:"s' \<in> learned r2 l"
-          with this obtain s'' where 4:"s'' \<preceq> s'" and 5:"s'' \<in> cgc_state.fromPrev r2" using inv4
-            by (auto simp add:inv4_def)
-          moreover
-          have "s \<preceq> s''" using 5 inv1 inv2 1 by (auto simp add:inv2_def inv1_def learn_def)
-          ultimately
-          show "compat2 s' s" using l1
-            by (metis compat_sym less_eq_def) 
-        qed
-        moreover
-        have "\<forall> s' \<in> cgc_state.toNext (refmap (r1, r2)) . s \<preceq> s'"
-        proof auto
-          fix s'
-          assume "s' \<in> cgc_state.toNext r2"
-          with this obtain s'' where 4:"s'' \<preceq> s'" and 5:"s'' \<in> cgc_state.fromPrev r2" using inv5
-            by (auto simp add:inv5_def)
-          have 6:"s \<preceq> s''" using 5 inv1 inv2 1 by (auto simp add:inv2_def inv1_def learn_def)
-          show "s \<preceq> s'" using 4 6
-            by (metis pre_CStruct.trans)
-        qed
-        ultimately
-        show ?thesis by (auto simp add:learn_def)
-      qed
-      thus ?thesis by (auto simp add:defs1 ref_defs)
-    qed next
+   apply (simp add:ref_defs spec_def actions_defs cgc_ioa_defs actions_defs inv_defs refmap_def non_trivial_def)
+   apply(split_conjs?)
+   apply (app_fun_eq_iff?, force?)
+   apply (metis Un_iff compat_sym l1 less_eq_def)
+   apply (metis pre_CStruct.trans)
+   apply (app_fun_eq_iff?, force?)
+
+   apply(rule_tac x="refmap (a,b)" in exI)
+   apply(rule_tac x="[(Learn2 x41 x42,refmap (aa,ba))]" in exI)
+   apply (simp add:ref_defs spec_def actions_defs cgc_ioa_defs actions_defs inv_defs refmap_def non_trivial_def)
+   apply(split_conjs?)
+   apply (insert l2)
+   apply (metis sup.mono)
+   apply (metis Un_iff l1)
+   apply (app_fun_eq_iff)
+
+   apply(rule_tac x="refmap (a,b)" in exI)
+   apply(rule_tac x="[]" in exI)
+   apply(force simp add:mydefs ref_defs refmap_def)
+
+   apply(rule_tac x="refmap (a,b)" in exI)
+   apply(rule_tac x="[(ToNext x6,refmap (aa,ba))]" in exI)
+   apply (simp add:ref_defs spec_def actions_defs cgc_ioa_defs actions_defs inv_defs refmap_def non_trivial_def)
+   apply(split_conjs?)
+   apply (insert l2)
+   apply (metis sup.mono)
+   apply (metis Un_iff less_eq_def pre_CStruct.trans)
+done
 
 lemma trace_incl:"traces composition \<subseteq> traces spec"
 apply(rule ref_map_soundness[of refmap])
-  defer
-  apply(simp add:defs1)
+  apply(insert refok, force)
+  apply(simp add:mydefs)
   apply(intro set_eqI; case_tac x; force)
-  apply(insert refok, auto)
 done
 
 theorem composition: "composition =<| spec"
 apply(simp add:ioa_implements_def)
 apply(intro conjI)
-  apply(simp add:defs1)
+  apply(simp add:mydefs)
   apply(intro set_eqI; case_tac x; force)
-  apply(simp add:defs1)
+  apply(simp add:mydefs)
   apply(intro set_eqI; case_tac x; force)
   apply (insert trace_incl, auto)
 done
